use the simpler BuildTree for real
(also fix termination of Match.btAt_newHist_length_eq_length_plus_oldHist)

Pdl/BuildTree.lean
@@ -15,312 +15,316 @@ Lessons learned while working on this file:
 
 -- See also Bml/CompletenessViaPaths.lean for inspiration that might be useful here.
 
+/-- A free repeat is a non-loaded sequent that occured before. -/
+def FreeRepeat (Hist : History) (X : Sequent) : Type :=
+  Subtype (fun k => (Hist.get k).multisetEqTo X ∧ ¬ X.isLoaded)
+
+mutual
 /-- Winning Strategy Tree for Builder.
-At a `BuStep` it is the turn of `Builder` and we have a single child for the `Move` they make.
-At a `PrStep` it is the turn of `Prover`, and we have children for all possible `Move`s.
+At each step, we consider
+- ALL rules R that prover may choose, followed immediately by
+- ONE of the children then chosen by Builder
 
-In the paper "a leaf is either labeled with a sequent to which no rule is applicable, or it is a
-(free) repeat". Here we make leafs with `PrStep` because at such a position it is the turn of Prover
-but there are no moves so Prover loses.
+The type is actually similar to `Tableau`, as it also uses a history, but it does allow open leaves.
+For choosing a local tableau end node the mutual `RuleChoice` is needed to avoid the error
+"nested inductive datatypes parameters cannot contain local variables".
+Instead of the .lpr constructor here we have .fpr because we only make a `RuleTree` when Builder
+wins and thus we can never reach an lpr where Prover would win, but do allow free repeats.
+As in `Tableau` note that the history is stored in reverse. -/
+inductive BuildTree : History → Sequent → Type
+  /-- Prover chooses local tab, we pick one end node. -/
+  | loc {H X} (nbas : ¬ X.basic)
+            (next : (lt : LocalTableau X) → BuildChoice H X (endNodesOf lt))
+            : BuildTree H X
+  /-- Prover chooses PDL rule, never branches, so continue with unique child. -/
+  | pdl {H X} (bas : X.basic)
+            (next : ∀ Y, ∀ _r : PdlRule X Y, BuildTree (X :: H) Y) : BuildTree H X
+  /-- Free repeat means builder wins. -/
+  | freeRepeat {H X} : FreeRepeat H X → BuildTree H X
+  /-- Leaf that is (might be?!) not a repeat, but no rules can be applied. -/
+  | openLeaf {H X} : BuildTree H X
+  -- TODO: add `(bas : X.basic)` for "no local rules" and somehow say "no PDL rules"?
+  -- small worry but what about (L+) (L-), one of which is always applicable?
+  -- Well, then it would lead to a free repeat!?
 
-GOAL: The `BuildTree` type should carry all information we need, so later we should not care
-about how a specific strategy tree for builder gets made/computed, but just that there is one.
+inductive BuildChoice : History → Sequent → List Sequent → Type
+  | pick {H X YS Y} : Y ∈ YS → BuildTree (X :: H) Y → BuildChoice H X YS
+end
 
-PROBLEM: This type currently makes too many steps where the sequence does not change.
-Note that Def 6.8. says that at every step a rule should be used!
-It seems that means we do not want the single-child `BuStep` here at all.???
+@[simp]
+lemma BuildChoice.fst_eq_H {H X YS} {bc : BuildChoice H X YS} : bc.1 = H := by
+  cases bc
+  rfl
 
-Each single step in the build tree should provide all three:
-- rule R chosen
-- child chosen
--/
-inductive BuildTree : GamePos → Type
-  | BuStep {pos newPos}
-      (hturn : tableauGame.turn pos = Builder)
-      (m : Move pos newPos)
-      (next : BuildTree newPos) -- single child
-      : BuildTree pos
-  | PrStep {pos}
-      (hturn : tableauGame.turn pos = Prover)
-      (next : ∀ newPos, ∀ _m : Move pos newPos, BuildTree newPos) -- all children
-      : BuildTree pos
-      -- side note: we no longer have a `List` here, so may need `Finset.sort (theMoves pos)`??
-
-def BuildTree.isLeaf {pos} : BuildTree pos → Prop
-  | BuildTree.BuStep .. => False
-  | BuildTree.PrStep .. => theMoves pos = ∅
-
-def BuildTree.isFreeRepLeaf {pos} : BuildTree pos → Prop
-  | BuildTree.BuStep .. => False
-  | @BuildTree.PrStep _ hturn _ =>
-      match pos with
-      | ⟨H, X, p⟩ =>
-        match p with
-        | .inl proPos =>
-          match proPos with
-            | .nlpRep _ _ => True -- free repeat!
-            | .bas _ _ => False -- might still be a Leaf, but not a repeat leaf
-            | .nbas _ _ => False -- not a leaf because prover can apply a local rule/tableau
-        | .inr _ => by exfalso; simp at hturn
-
-theorem BuildTree.rep_of_isFreeRepLeaf {pos : GamePos} {bt : BuildTree pos} :
-    bt.isFreeRepLeaf → rep pos.1 pos.2.1 := by
-  intro h
-  unfold isFreeRepLeaf at h
-  rcases pos with ⟨H, X, p⟩
-  cases bt <;> simp at *
-  case PrStep hturn next =>
-    cases p <;> simp at *
-    case inl proPos =>
-      cases proPos <;> simp at *
-      case nlpRep theRep lpr => exact theRep
-    · exfalso; grind
-
-/-- TODO: `BuildTree.isLeaf` implies that either we have a free repeat or we have a
-basic sequence to which no rule can be applied (and that is easily satisfiable?) -/
-theorem BuildTree.isLeaf_iff {pos} {bt : BuildTree pos} :
-    bt.isLeaf → bt.isFreeRepLeaf ∨ pos.2.1.basic := by
-  intro bt_isLeaf
-  cases bt
-  case BuStep newPos next hturn m =>
-    unfold isLeaf at bt_isLeaf
-    simp at *
-  case PrStep =>
-    unfold isLeaf at bt_isLeaf
-    simp only at *
-
-    sorry
-
-/-- Given a winning Builder strategy, compute its `BuildTree`. -/
-def buildTree (s : Strategy tableauGame Builder) {H X p} (h : winning s ⟨H, X, p⟩) :
-    BuildTree ⟨H, X, p⟩ :=
+/-- Given a winning Builder strategy, compute its `RuleTree`.
+NEW: note the `Sum.inl p` here. This ensure we start tree building from a Prover position, i.e.
+- not allowing BuilderPos.lpr here (easy, was forbidden already anyway as prover wins there.)
+- not allowing BuilderPos.ltab because we cannot use BuildTree.loc for a single fixed local tab. -/
+def buildTree (s : Strategy tableauGame Builder) {H X p} (h : winning s ⟨H, X, Sum.inl p⟩) :
+    BuildTree H X :=
   match p_def : p with
   -- Prover positions:
-  | Sum.inl (.nlpRep rp noLpRep) => .PrStep (by simp) (by intro _ m; cases m) -- Builder wins rep.
-  | Sum.inl (.bas nrep bas) => -- prover chooses PDL rule
+  | (.nlpRep rp noLpRep) => .openLeaf -- Builder wins rep. ?? maybe we do want history?
+  | (.bas nrep bas) => -- prover chooses PDL rule
       have stillWin : ∀ newP, ∀ _ : Move ⟨_,_,Sum.inl (.bas nrep bas)⟩ newP, winning s newP :=
         fun newPos mov =>
           @winning_of_whatever_other_move _ _ s _ (by simp) h ⟨newPos, mem_theMoves_of_move ⟨mov⟩⟩
-      @BuildTree.PrStep ⟨_,_,Sum.inl (.bas nrep bas)⟩ (by simp_all)
-        (fun newPos mov => buildTree s (stillWin newPos mov))
-  | Sum.inl (.nbas nrep nbas) => -- prover chooses a local tableau
+      .pdl bas <| fun newSeq r => by
+        -- deal with the result of `posOf` here already because we can only make a
+        -- recursive call if we again have a ProverPos.
+        cases newPos_def : posOf (X :: H) newSeq
+        case inl newP =>
+          have _forTermination : Relation.TransGen tableauGame.wf.1 ⟨_,_, .inl newP⟩ ⟨_,_, .inl p⟩
+            := by rw [p_def, ← newPos_def]; exact Relation.TransGen.single ⟨Move.prPdl r⟩
+          refine @buildTree s (X :: H) newSeq newP (stillWin ⟨_, _, Sum.inl newP⟩ ?_)
+          rw [← newPos_def]
+          exact @Move.prPdl _ _ H nrep bas r
+        case inr newBP =>
+          exfalso
+          -- IDEA: The only BuilderPos resulting from `posOf` is an lpr ...
+          rcases posOf_eq_inr_then_lpr newPos_def with ⟨lpr, newBP_def⟩
+          have := stillWin ⟨_, _, posOf (X :: H) newSeq⟩ (Move.prPdl r)
+          rw [newPos_def, newBP_def] at this
+          -- .. where prover would win, so that cannot happen here.
+          simp [winning] at this
+  | (.nbas nrep nbas) => -- prover chooses a local tableau
       have stillWin : ∀ newP, ∀ _ : Move ⟨_,_,Sum.inl (.nbas nrep nbas)⟩ newP, winning s newP :=
         fun newPos mov =>
           @winning_of_whatever_other_move _ _ s _ (by simp) h ⟨newPos, mem_theMoves_of_move ⟨mov⟩⟩
-      @BuildTree.PrStep ⟨_,_,Sum.inl (.nbas nrep nbas)⟩ (by simp_all)
-        (fun newPos mov => buildTree s (stillWin newPos mov))
-  -- Builder positions:
-  | Sum.inr (.lpr _) => by exfalso; simp [winning] at h -- prover wins, cannot happen
-  | Sum.inr (.ltab nrep nbas ltX) =>
-      if ne : (tableauGame.moves ⟨H, ⟨X, Sum.inr (BuilderPos.ltab nrep nbas ltX)⟩⟩).Nonempty
-      then
-        -- Builder can use `s` to choose some `Y ∈ endNodeOf ltX`.
-        let sY := (s ⟨H, X, Sum.inr (.ltab nrep nbas ltX)⟩ (by simp) ne)
-        have Mov : Move ⟨H, X, Sum.inr (.ltab nrep nbas ltX)⟩ sY.1 := by
-          have := sY.2
-          simp only [Game.Pos.moves, tableauGame, theMoves, List.mem_toFinset] at this
-          simp [List.mem_map] at this
-          let oY := List.find? -- No more choice thanks to this!
-            (fun Y => @decide (⟨X :: H, ⟨Y, posOf (X :: H) Y⟩⟩ = sY.val) (instDecidableEqPos _ _))
-            (endNodesOf ltX)
-          cases oY_def : oY
-          · exfalso
-            have := List.find?_eq_none.mp oY_def
+      .loc nbas <| fun ltX => by
+        have ne : (tableauGame.moves ⟨H, ⟨X, Sum.inr (BuilderPos.ltab nrep nbas ltX)⟩⟩).Nonempty :=
+          winning_has_moves (by simp) <|
+            stillWin ⟨H, ⟨X, Sum.inr (BuilderPos.ltab nrep nbas ltX)⟩⟩ Move.prLocTab
+        -- IDEA: use strategy `s` to choose move `mY` that picks the `Y ∈ endNodeOf ltX`:
+        -- We want to define mY and then do rcases, but keep the information how it was defined.
+        let mY_raw := s ⟨H, X, Sum.inr (.ltab nrep nbas ltX)⟩ (by simp) ne
+        have mY_def : mY_raw.1 = s ⟨H, X, Sum.inr (.ltab nrep nbas ltX)⟩ (by simp) ne := rfl
+        rcases mY_raw with ⟨mY, mY_prop⟩
+        simp at mY_def
+        -- We continue the BuildTree with the chosen `Y`:
+        refine (@BuildChoice.pick _ _ _ mY.2.1 ?in_endNodesOf_ltX ?subtree_for_mY)
+        · have := mY_prop
+          unfold Game.Pos.moves Game.moves tableauGame at this
+          simp only at this
+          rw [theMoves_iff] at this
+          simp at this
+          rcases this with ⟨_,_,⟨Y',Y'_in,mY_def⟩⟩
+          rw [mY_def]
+          simp
+          exact Y'_in
+        · -- now still need to make a `Move` so we can recursively call `buildTree`.
+          have Mov : Move ⟨H, X, Sum.inr (.ltab nrep nbas ltX)⟩ mY := by
+            simp only [Game.Pos.moves, tableauGame, theMoves, List.mem_toFinset] at mY_prop
+            simp [List.mem_map] at mY_prop
+            let oY := List.find? -- No more choice thanks to this!
+              (fun Y => @decide (⟨_, ⟨_, posOf (X :: H) Y⟩⟩ = mY) (instDecidableEqPos _ _))
+              (endNodesOf ltX)
+            cases oY_def : oY
+            · exfalso
+              have := List.find?_eq_none.mp oY_def
+              grind
+            case some Y =>
+              unfold oY at oY_def
+              have def_mY := List.find?_some oY_def
+              simp only [decide_eq_true_eq] at def_mY
+              have Y_in := List.mem_of_find?_eq_some oY_def
+              have := @Move.buEnd X ltX Y H nrep nbas Y_in
+              rw [← def_mY]
+              exact this
+          rcases mY with ⟨H', Y, newP⟩ -- Happy because this does not lose mY_def.
+          have H'_def : H' = X :: H := by
+            simp [Game.Pos.moves, tableauGame, Game.moves] at mY_prop
             grind
-          case some Y =>
-            unfold oY at oY_def
-            have def_sY := List.find?_some oY_def
-            simp only [decide_eq_true_eq] at def_sY
-            have Y_in := List.mem_of_find?_eq_some oY_def
-            have := @Move.buEnd X ltX Y H nrep nbas Y_in
-            rw [← def_sY]
-            exact this
-        have stillWin : winning s sY.1 := winning_of_winning_move _ h
-        have forTermination : move ⟨H, X, Sum.inr (.ltab nrep nbas ltX)⟩ sY.1 := ⟨Mov⟩ -- needed?
-        BuildTree.BuStep (by simp) Mov (buildTree s stillWin)
-      else by
-        exfalso
-        simp_all [winning, winner]
+          -- Case distinction here to ensure newP from mY is a ProverPos for recursion.
+          match newP with
+          | .inl myP =>
+            simp only
+            -- Make recursive call:
+            have _forTermination : Relation.TransGen tableauGame.wf.1 ⟨_,_, .inl myP⟩ ⟨_,_, .inl p⟩
+              :=  by
+                unfold WellFoundedRelation.rel Game.wf tableauGame
+                simp
+                apply @Relation.TransGen.trans _ _ _
+                  ⟨H, ⟨X, Sum.inr (BuilderPos.ltab nrep nbas ltX)⟩⟩
+                · exact Relation.TransGen.single ⟨Mov⟩
+                · rw [p_def]; exact Relation.TransGen.single ⟨Move.prLocTab⟩
+            refine H'_def ▸ @buildTree s H' Y myP ?_
+            -- (Remaining goal is nicer after doing `H'_def ▸` on the outside and not on `myP`.)
+            rw [mY_def]
+            -- Note that *two* moves have happened now, one by prover and one by Builder using `s`.
+            -- Remains to show that `s` still wins.
+            apply winning_of_winning_move
+            exact stillWin ⟨_, X, Sum.inr (BuilderPos.ltab nrep nbas ltX)⟩ Move.prLocTab
+          | .inr mY_BP =>
+              exfalso -- fingers crossed ;-)
+              subst H'_def
+              -- (This is different than above, cannot use `posOf_eq_inr_then_lpr` immediately.)
+              -- OLD IDEA: mY is result of Move.buEnd, so if mY is a BuilderPos then it is an lpr.
+              -- cannot do `cases Mov` -- Dependent elimination failed: Failed to solve equation
+              -- `Mov` goes from a BuilderPos.ltab to `mY_BP`, so `mY_BP` must be a `posOf` result.
+              -- Distinguish cases what the BP we reach can be.
+              cases mY_BP
+              case lpr lr => -- possible
+                suffices winning s ⟨X :: H, ⟨Y, Sum.inr (BuilderPos.lpr lr)⟩⟩ by
+                  simp [winning] at this
+                rw [mY_def]
+                apply @winning_of_winning_move _ _ s
+                exact stillWin ⟨_, X, Sum.inr (BuilderPos.ltab nrep nbas ltX)⟩ Move.prLocTab
+              case ltab => -- impossible
+                clear mY_def mY_prop newP
+                have := mem_theMoves_of_move (⟨Mov⟩)
+                absurd this
+                simp [theMoves]
+                intro Z Z_in
+                have := endNodesOf_basic Z_in
+                grind
 termination_by
-  tableauGame.wf.2.wrap (⟨H, X, p⟩ : GamePos)
-decreasing_by -- show that it's a move
-  · simp_wf
-    simp only [tableauGame, Game.wf, WellFoundedRelation.rel]
-    exact ⟨mov⟩
-  · simp_wf
-    simp only [tableauGame, Game.wf, WellFoundedRelation.rel]
-    exact ⟨mov⟩
-  · simp_wf
-    simp only [tableauGame, Game.wf, WellFoundedRelation.rel]
-    exact forTermination
+  -- Might need 2 moves, so we use the transitive closure (which is still wellfounded)
+  tableauGame.wf.2.transGen.wrap (⟨H, X, Sum.inl p⟩ : GamePos)
+decreasing_by
+  all_goals
+    simp_wf
+    rw [← p_def]
+    exact _forTermination
 
 /-! ## Matches -/
 
 /-- A match is a path inside a `BuildTree`. Analogous to `PathIn` for `Tableau`. In Game Theory
-this could be called a "rollout", but note that it stays within the given Builder strategy tree. -/
-inductive Match : ∀ {pos : GamePos}, BuildTree pos → Type
+this could be called a "rollout", but note that it stays within the given Builder strategy tree
+and it is not tracking all intermediate game positions. -/
+inductive Match : ∀ {H : History} {X : Sequent}, BuildTree H X → Type
   | nil {bt} : Match bt
-  | bu : Match next → Match (BuildTree.BuStep hturn m next)
-  | pr newPos :
-      (mov : Move pos newPos)
-      → Match (next newPos mov) → Match (@BuildTree.PrStep pos hturn next)
+  | loc {nbas next lt} : Match (next lt).6 → Match (BuildTree.loc nbas next)
+  | pdl {bas next Y r} : Match (next Y r) → Match (BuildTree.pdl bas next)
 
 /-
--- TODO, use `LocalAll` and `AllPdlRule`
+-- TODO, but NOW do not use `LocalAll` and `AllPdlRule` for this probably.
 -- Wait, where are these actually used at the moment or will they be needed later?
 
-def BuildTree.all_Match (bt : BuildTree pos) : List (Match bt) := sorry
+def BuildTree.all_Match (bt : BuildTree X) : List (Match bt) := sorry
 
-theorem BuildTree.all_Match_spec (bt : BuildTree pos) :
+theorem BuildTree.all_Match_spec (bt : BuildTree X) :
     ∀ m, m ∈ bt.all_Match := by
   sorry
 -/
 
-/-- Inspired by `PathIn.length`.
-Note that this counts all steps, even the `prLocTab` ones where `pos.1` does not get longer. -/
+/-- Inspired by `PathIn.length`. Counting the steps made by a `Match` in a `BuildTree`.
+Note that such a step may be combinations of a prover and a builder move. -/
 @[simp]
-def Match.length {pos : GamePos} {bt : BuildTree pos} : Match bt → Nat
+def Match.length {H : History} {X : Sequent} {bt : BuildTree H X} : Match bt → Nat
   | .nil => 0
-  | .bu tail => tail.length + 1
-  | .pr _ _ tail => tail.length + 1
+  | .loc tail => tail.length + 1
+  | .pdl tail => tail.length + 1
 
-def Match.btAt {pos} {bt : BuildTree pos} : Match bt → Σ newPos, BuildTree newPos
-| .nil => ⟨_, bt⟩
-| .bu tail => btAt tail
-| .pr _ _ tail => btAt tail
+def Match.btAt {H X} {bt : BuildTree H X} : Match bt → Σ H' Y, BuildTree H' Y
+| .nil => ⟨_, _, bt⟩
+| .loc tail => btAt tail
+| .pdl tail => btAt tail
 
 -- TODO lemmas like those about `tabAt` and `nodeAt`?
 
-def Match.append : (m1 : Match bt) → (m2 : Match (btAt m1).2) → Match bt
+def Match.append {H X} {bt : BuildTree H X} :
+    (m1 : Match bt) → (m2 : Match (btAt m1).2.2) → Match bt
 | .nil, m2 => m2
-| .bu tail, m2 => .bu (append tail m2)
-| .pr _ _ tail, m2 => .pr _ _ (append tail m2)
+| .loc tail, m2 => .loc (append tail m2)
+| .pdl tail, m2 => .pdl (append tail m2)
 
 -- TODO lemmas like those about `PathIn.append`?
 
-structure Match.BuEdge (m n : Match bt) where
-  mPos : GamePos
-  hturn : tableauGame.turn mPos = Builder
-  mov : Move mPos n.btAt.1
-  h : btAt m = ⟨mPos, @BuildTree.BuStep _ _ hturn mov (btAt n).2⟩
+@[grind]
+structure Match.locEdge (m n : Match bt) where
+  H : History
+  mY : Sequent
+  nbas : _
+  next : (lt : LocalTableau mY) → BuildChoice H mY (endNodesOf lt)
+  lt : LocalTableau mY
+  btAt_m_def : btAt m = ⟨H, mY, @BuildTree.loc _ mY nbas next⟩
+  btAt_n_def : btAt n = ⟨(next lt).2 :: (next lt).1, (next lt).4, (next lt).6⟩
 
-structure Match.PrEdge (m n : Match bt) where
-  mPos : GamePos
-  hturn : tableauGame.turn mPos = Prover
-  mov : Move mPos n.btAt.1
-  next : _
-  btAt_m_def : btAt m = ⟨mPos, @BuildTree.PrStep _ hturn next⟩
-  next_n_def : next (btAt n).1 n_in = (btAt n).2
+@[grind]
+structure Match.pdlEdge (m n : Match bt) where
+  H : History
+  mX : Sequent
+  nY : Sequent
+  bas : mX.basic
+  next : ∀ Y, ∀ _r : PdlRule mX Y, BuildTree (mX :: H) Y
+  r : PdlRule mX nY
+  btAt_m_def : btAt m = ⟨_, mX, @BuildTree.pdl H mX bas next⟩
+  btAt_n_def : btAt n = ⟨_, _, next nY r⟩
 
 /-- The parent-child relation ⋖_𝕋 in a Builder strategy tree. -/
-def Match.Edge (m n : Match bt) : Type := Match.BuEdge m n ⊕ Match.PrEdge m n
+def Match.Edge (m n : Match bt) : Type := Match.locEdge m n ⊕ Match.pdlEdge m n
 
 /-- This edge between matches is a modal step.
-To even say this `BuildTree` must contain `Move` and thus rule data. -/
-def Match.Edge.isModal {pos} {bt : BuildTree pos} {m n : Match bt} : Match.Edge m n → Prop :=
-  match btAt_m_def : btAt m with
-  | ⟨⟨Hist, X, p⟩, m_bt⟩ =>
-    fun m_n =>
-      match m_bt with
-      | @BuildTree.BuStep _ p YS next YS_moves => False -- Builder moves are never modal steps.
-      | .PrStep hturn next =>
-        match m_n with
-        | .inl m_bu_n => by exfalso; grind [BuEdge]
-        | .inr m_pr_n => m_pr_n.mov.isModal
+To even say this `BuildTree` must contain the rule data. -/
+def Match.Edge.isModal {H X} {bt : BuildTree H X} {m n : Match bt} : Match.Edge m n → Prop
+  | Sum.inl _ => False -- local edges are never modal steps.
+  | Sum.inr ⟨_, _, _, _, _, r, _, _⟩ =>  PdlRule.isModal r
 
-def Match.isLeaf {pos} {bt : BuildTree pos} {m : Match bt} : Prop := (btAt m).2.isLeaf
+def Match.isLeaf {H X} {bt : BuildTree H X} {m : Match bt} : Prop :=
+  match (btAt m) with | ⟨_, _, .openLeaf⟩ => True | _ => False
 
 /-- If `m` ends at a leaf, then it cannot have an edge to any `n`. -/
-lemma Match.isLeaf_no_edge {bt : BuildTree pos} (m : Match bt) (h : m.isLeaf) :
-    ∀ n, ¬ Nonempty (Match.Edge m n) := by
+lemma Match.isLeaf_no_edge {H X} {bt : BuildTree H X} (m : Match bt) (h : m.isLeaf) :
+    ∀ n, ¬ Nonempty (Match.Edge m n) := by -- EASY as expected :)
   intro n
   unfold Match.isLeaf at h
-  by_contra hyp
-  rcases hyp with ⟨m_bu_n|m_pr_n⟩
-  · grind [BuildTree.isLeaf, Match.BuEdge]
-  · simp only [BuildTree.isLeaf] at h
-    rcases m_pr_n with ⟨mPos, hturn, mov, next, btAt_m_def, next_n_def⟩
-    have := @mem_theMoves_of_move mPos n.btAt.1 ⟨mov⟩
-    grind
+  rintro ⟨m_n⟩
+  cases m_n <;> grind
 
-/-- Convert a `Match` to a `History`. Inspired by `PathIn.toHistory`.
-Does not include the last node.
-The history of `.nil` is `[]` because this will not go into `pos.1`.
-IDEA: only record the .pr steps here, but skip .bu steps?!
--/
-def Match.toHistory {pos : GamePos} {bt : BuildTree pos} : (m : Match bt) → History
-| .nil => []
-| .bu tail => tail.toHistory ++ [pos.2.1]
-| .pr _ _ tail => tail.toHistory ++ [pos.2.1]
+-- Maybe Match.toHistory is not actually needed? Skipping it for now.
 
 /-- Rewind a `Match`, i.e. go back up inside `bt` by `k` steps.
-This used to use `Nat` but now we take a `Fin` like in `PathIn.rewind`, and
-for that we needed to define `Match.length` first.
-IDEA: also use `Match.toHistory` here? -/
-def Match.rewind {pos} {bt : BuildTree pos} : (m : Match bt) → (k : Fin (m.length + 1)) → Match bt
-| .nil, _ => .nil
-| .bu tail, k => Fin.lastCases (.nil) (Match.bu ∘ tail.rewind) k
-| .pr _ _ tail, k => Fin.lastCases (.nil) (Match.pr _ _ ∘ tail.rewind) k
+The + 1 is there because going back 0 steps does nothing. -/
+def Match.rewind {H X} {bt : BuildTree H X} : (m : Match bt) → (k : Fin (m.length + 1)) → Match bt
+| .nil, 0 => .nil
+| .nil, ⟨k+1,k_h⟩ => by exfalso; simp at k_h
+| .loc tail, k => Fin.lastCases (.nil) (Match.loc ∘ tail.rewind) k
+| .pdl tail, k => Fin.lastCases (.nil) (Match.pdl ∘ tail.rewind) k
 
--- ... lots of stuff needed here?
+-- move up later?
+def BuildTree.isFreeRepeat {H X} : BuildTree H X → Prop
+  | BuildTree.freeRepeat _ => True
+  | _ => False
 
-/-- The extra condition that it is the turn of Builder is needed because otherwise
-the `prLocTab` case would falsify. -/
-theorem Move.fst_length_succ {H X p} (mov : Move ⟨H, ⟨X, p⟩⟩ newPos) :
-    tableauGame.turn ⟨H, ⟨X, p⟩⟩ = Builder →
-    newPos.1.length = H.length + 1 := by
-  cases mov <;> simp
+def BuildTree.getFreeRepeat {H X} {bt : BuildTree H X}
+    (h : bt.isFreeRepeat) : FreeRepeat H X := by
+  unfold isFreeRepeat at h
+  cases bt <;> simp at *
+  case freeRepeat fr => exact fr
 
-/-- This is NOT TRUE, because history only records different steps and will
-*not* count `Move.prLocTab` steps, though these are steps in the `Match`.
+lemma Match.btAt_newHist_length_eq_length_plus_oldHist {H X} {bt : BuildTree H X} (m : Match bt) :
+    m.btAt.1.length = m.length + H.length :=
+  match m with
+  | nil => by simp [btAt]
+  | @loc _ _ _ next lt tail => by
+    have IH := Match.btAt_newHist_length_eq_length_plus_oldHist tail
+    unfold btAt
+    rw [IH]
+    simp
+    grind
+  | pdl tail => by
+    have IH := Match.btAt_newHist_length_eq_length_plus_oldHist tail
+    simp
+    unfold btAt
+    rw [IH]
+    simp
+    omega
+termination_by
+  m.length
 
-WAIT, but `Match.toHistory` DOES count all steps, so the length statement here should be true. ??
-
-?? are we sure about this one ??
-Note that the history from `pos` needs to be added on the right side.
-
-?? Or better restrict `pos` to be a *starting* position of the game!?!?
-(Analogous to how many things in TableauPath are only the `Hist = []` case.) -/
-theorem Match.btAt_fst_fst_length_eq_length {bt : BuildTree pos} {m : Match bt} :
-    m.btAt.1.1.length = m.length + pos.1.length := by
-  induction bt
-  case BuStep pos newPos hturn mov next IH =>
-    cases m
-    case nil =>
-      rcases pos with ⟨H, X, p⟩
-      simp [Match.btAt]
-    case bu hturn tail =>
-      -- FIXME: change defs above to avoid duplicate `hturn` here?!
-      rcases pos with ⟨H, X, p⟩
-      simp [Match.btAt]
-      specialize @IH tail
-      rw [add_assoc]
-      convert IH using 2
-      grind [Move.fst_length_succ mov]
-  case PrStep pos hturn next IH =>
-    cases m
-    case nil =>
-      rcases pos with ⟨H, X, p⟩
-      simp [Match.btAt]
-    case pr newPos hturn mov tail =>
-      rcases pos with ⟨H, X, p⟩
-      simp [Match.btAt]
-      specialize @IH _ mov tail
-      rw [add_assoc]
-      convert IH using 2
-      -- NOT provable here because `newPos.1` is a history not counting `prLocTab` steps,
-      -- whereas the H list coming from `Match.toHistory` does count them.
-      sorry
-
-def Match.companionOf {bt : BuildTree pos} (m : Match bt)
-  (h : (btAt m).2.isFreeRepLeaf) : Match bt :=
-    -- WAS: m.rewind (theRep ((btAt m).2.rep_of_isFreeRepLeaf h))
-    -- WANT: m.rewind (rep.toFin ((btAt m).2.rep_of_isFreeRepLeaf h))
-    sorry
+/-- Roll back to the companion. Only possibe if we started with H=[] so we know the root. -/
+def Match.companionOf {X} {bt : BuildTree [] X} (m : Match bt)
+  (h : (btAt m).2.2.isFreeRepeat) : Match bt :=
+    match BuildTree.getFreeRepeat h with
+    -- The free repeat says "go k steps back" where k < length of history at `m`.
+    | ⟨⟨k, k_lt⟩ , same_and_free⟩ =>
+      -- But to rewind m we need a k < length of m itself plus 1
+      m.rewind ⟨k, by grind [Match.btAt_newHist_length_eq_length_plus_oldHist]⟩
 
 /-- The repeat ♥ companion relation on `Match`. -/
-def Match.companion (m n : Match bt) : Prop :=
-  ∃ (h : (btAt m).2.isFreeRepLeaf), n = Match.companionOf m h
+def Match.companion {X} {bt : BuildTree [] X} (m n : Match bt) : Prop :=
+  ∃ (h : (btAt m).2.2.isFreeRepeat), n = Match.companionOf m h
 
 local notation ma:arg " ♥ " mb:arg => Match.companion ma mb
 
@@ -336,38 +340,38 @@ we only store the π part of such pre-states, because the π' is then uniquely d
 
 /-- A pre-state-part starting at `m` is any path in `bt : BuildTree` consisting of non-(M) `edge`s
 and stopping at a leaf or at an (M) application. (No `Match.companion` steps here, see note above.)
-
-PROBLEM / QUESTION: do we also need leafs given by empty `prMoves`??? -/
-inductive PreStateP {pos} (bt : BuildTree pos) : (m : Match bt) → Type
+-/
+inductive PreStateP {H X} (bt : BuildTree H X) : (m : Match bt) → Type
 | edge {m n} : (e : Match.Edge m n) → ¬ e.isModal → PreStateP bt n → PreStateP bt m
 | stopLeaf {m} : m.isLeaf → PreStateP bt m
 | stopAtM {m n} : (e : Match.Edge m n) → e.isModal → PreStateP bt m
 
 /-- Collect all `PreStateP`s from a given `m` onwards. -/
-def BuildTree.allPreStatePs {pos} : (bt : BuildTree pos) → (m : Match bt) → List (PreStateP bt m)
-  -- Maybe define `Match.all` first and then filter it here?
-  -- Or better do it inductively?
-| .PrStep hturn next, m => sorry
-    -- [ .stopLeaf (by unfold Match.isLeaf; cases m; simp_all [Match.btAt]) ]
-| .BuStep hturn mov next, _ => sorry
+-- Maybe define `Match.all` first and then filter it here?
+-- Or better do it inductively?
+def BuildTree.allPreStatePs {H X} : (bt : BuildTree H X) → (m : Match bt) → List (PreStateP bt m)
+| .loc nbas next, m => sorry
+| .pdl bas next, _ => sorry
+| .freeRepeat fr, m => sorry
+| .openLeaf, m => sorry
 
-lemma BuildTree.allPreStatePs_spec {pos} {bt : BuildTree pos} {m : Match bt} :
+lemma BuildTree.allPreStatePs_spec {H X} {bt : BuildTree H X} {m : Match bt} :
     ∀ π : PreStateP bt m, π ∈ bt.allPreStatePs m := by
   sorry
 
 /-- A pre-state is a maximal pre-state-part, i.e. starting at the root or just after (M).
 
-WORRY: should `fromRoot` also have a condition about `pos` being the start of the game?
+WORRY: should `fromRoot` also have a condition about `H` being empty, i.e. the start of the game?
 -/
-inductive PreState {pos} (bt : BuildTree pos) : Type
+inductive PreState {H X} (bt : BuildTree H X) : Type
 | fromRoot : PreStateP bt .nil → PreState bt
 | fromMod {o m} : (e : Match.Edge o m) → e.isModal → PreStateP bt m → PreState bt
 
 /-- Collect all `PreState`s for a given `BuildTree`. -/
-def BuildTree.allPreStates {pos} (bt : BuildTree pos) : List (PreState bt) :=
+def BuildTree.allPreStates {H X} (bt : BuildTree H X) : List (PreState bt) :=
   (bt.allPreStatePs .nil).map .fromRoot
 
-lemma BuildTree.allPreStates_spec {pos} {bt : BuildTree pos} :
+lemma BuildTree.allPreStates_spec {H X} {bt : BuildTree H X} :
     ∀ π : PreState bt, π ∈ bt.allPreStates := by
   -- should be easy, use BuildTree.allPreStatePs_spec
   sorry
@@ -408,7 +412,8 @@ lemma PreState.locConsSatBas (π : PreState bt) :
 
 /-- Definition 6.17 to get model graph from strategy tree. -/
 @[simp]
-def BuildTree.toModel (bt : BuildTree Pos) : (Σ W : Finset (Finset Formula), KripkeModel W) :=
+def BuildTree.toModel {H X} (bt : BuildTree H X) :
+    (Σ W : Finset (Finset Formula), KripkeModel W) :=
   ⟨ ((bt.allPreStates).map (List.toFinset ∘ PreState.forms)).toFinset -- W
   , { val := fun X p => Formula.atom_prop p ∈ X.1 -- valuation V(p)
     , Rel := fun a X Y => -- relation Rₐ
@@ -421,7 +426,7 @@ QUESTION: which `R` can we use here in order to use `Modelgraphs.Q`?
 lemma PreState.diamondExistence {φ : AnyFormula} {π : PreState bt} : (~'⌊α⌋φ) ∈ π.lforms →
     -- QUESTION: what to say about `π` here and what to say about node `t` lying on `π`?
     ∃ t : Match bt,
-        AnyNegFormula.mem_Sequent (t.btAt).1.2.1 (~''φ)
+        AnyNegFormula.mem_Sequent (t.btAt).2.1 (~''φ)
       ∧ ∃ ρ : PreState bt, ∃ u : Match bt,
         -- TODO: t < u
         -- TODO: missing loaded formulas below
@@ -434,10 +439,13 @@ lemma PreState.diamondExistence {φ : AnyFormula} {π : PreState bt} : (~'⌊α�
 
 /-! ## Model graph of pre-states -/
 
-/-- Theorem 6.21: If Builder has a winning strategy then there is a model graph. -/
+/-- Theorem 6.21: If Builder has a winning strategy then there is a model graph.
+Uses `BuildTree.toModel`. -/
 theorem strmg (X : Sequent) (s : Strategy tableauGame Builder) (h : winning s (startPos X)) :
     ∃ (WS : Finset (Finset Formula)) (mg : ModelGraph WS), ∃ Z ∈ WS, X.toFinset ⊆ Z := by
-  let bt := buildTree s h
+  unfold startPos at h
+  rcases posOf_for_startPos X with ⟨proPos, posOf_def⟩
+  let bt := buildTree s (posOf_def ▸ h)
   let WS := bt.toModel.1
   let M := bt.toModel.2
   refine ⟨WS, ⟨M, ⟨?a, ?b, ?c, ?d⟩⟩, ?X_in⟩
