Unused/BuildTreeOld.lean
@@ -1,0 +1,472 @@
+import Pdl.TableauGame
+import Pdl.AllPdlRule
+
+/-! # From winning strategies to model graphs (Section 6.3)
+
+Lessons learned while working on this file:
+
+- Not all leafs in the BuildTree are backpointers.
+  We want open leafs (where builder wins the game) to actually build worlds :-)
+  Moreover, free repeats also let builder win.
+
+-/
+
+/-! ## BuildTree -/
+
+-- See also Bml/CompletenessViaPaths.lean for inspiration that might be useful here.
+
+/-- Winning Strategy Tree for Builder.
+At a `BuStep` it is the turn of `Builder` and we have a single child for the `Move` they make.
+At a `PrStep` it is the turn of `Prover`, and we have children for all possible `Move`s.
+
+In the paper "a leaf is either labeled with a sequent to which no rule is applicable, or it is a
+(free) repeat". Here we make leafs with `PrStep` because at such a position it is the turn of Prover
+but there are no moves so Prover loses.
+
+GOAL: The `BuildTree` type should carry all information we need, so later we should not care
+about how a specific strategy tree for builder gets made/computed, but just that there is one.
+
+PROBLEM: This type currently makes too many steps where the sequence does not change.
+Note that Def 6.8. says that at every step a rule should be used!
+It seems that means we do not want the single-child `BuStep` here at all.???
+
+Each single step in the build tree should provide all three:
+- rule R chosen
+- child chosen
+-/
+inductive BuildTree : GamePos → Type
+  | BuStep {pos newPos}
+      (hturn : tableauGame.turn pos = Builder)
+      (m : Move pos newPos)
+      (next : BuildTree newPos) -- single child
+      : BuildTree pos
+  | PrStep {pos}
+      (hturn : tableauGame.turn pos = Prover)
+      (next : ∀ newPos, ∀ _m : Move pos newPos, BuildTree newPos) -- all children
+      : BuildTree pos
+      -- side note: we no longer have a `List` here, so may need `Finset.sort (theMoves pos)`??
+
+def BuildTree.isLeaf {pos} : BuildTree pos → Prop
+  | BuildTree.BuStep .. => False
+  | BuildTree.PrStep .. => theMoves pos = ∅
+
+def BuildTree.isFreeRepLeaf {pos} : BuildTree pos → Prop
+  | BuildTree.BuStep .. => False
+  | @BuildTree.PrStep _ hturn _ =>
+      match pos with
+      | ⟨H, X, p⟩ =>
+        match p with
+        | .inl proPos =>
+          match proPos with
+            | .nlpRep _ _ => True -- free repeat!
+            | .bas _ _ => False -- might still be a Leaf, but not a repeat leaf
+            | .nbas _ _ => False -- not a leaf because prover can apply a local rule/tableau
+        | .inr _ => by exfalso; simp at hturn
+
+theorem BuildTree.rep_of_isFreeRepLeaf {pos : GamePos} {bt : BuildTree pos} :
+    bt.isFreeRepLeaf → rep pos.1 pos.2.1 := by
+  intro h
+  unfold isFreeRepLeaf at h
+  rcases pos with ⟨H, X, p⟩
+  cases bt <;> simp at *
+  case PrStep hturn next =>
+    cases p <;> simp at *
+    case inl proPos =>
+      cases proPos <;> simp at *
+      case nlpRep theRep lpr => exact theRep
+    · exfalso; grind
+
+/-- TODO: `BuildTree.isLeaf` implies that either we have a free repeat or we have a
+basic sequence to which no rule can be applied (and that is easily satisfiable?) -/
+theorem BuildTree.isLeaf_iff {pos} {bt : BuildTree pos} :
+    bt.isLeaf → bt.isFreeRepLeaf ∨ pos.2.1.basic := by
+  intro bt_isLeaf
+  cases bt
+  case BuStep newPos next hturn m =>
+    unfold isLeaf at bt_isLeaf
+    simp at *
+  case PrStep =>
+    unfold isLeaf at bt_isLeaf
+    simp only at *
+
+    sorry
+
+/-- Given a winning Builder strategy, compute its `BuildTree`. -/
+def buildTree (s : Strategy tableauGame Builder) {H X p} (h : winning s ⟨H, X, p⟩) :
+    BuildTree ⟨H, X, p⟩ :=
+  match p_def : p with
+  -- Prover positions:
+  | Sum.inl (.nlpRep rp noLpRep) => .PrStep (by simp) (by intro _ m; cases m) -- Builder wins rep.
+  | Sum.inl (.bas nrep bas) => -- prover chooses PDL rule
+      have stillWin : ∀ newP, ∀ _ : Move ⟨_,_,Sum.inl (.bas nrep bas)⟩ newP, winning s newP :=
+        fun newPos mov =>
+          @winning_of_whatever_other_move _ _ s _ (by simp) h ⟨newPos, mem_theMoves_of_move ⟨mov⟩⟩
+      @BuildTree.PrStep ⟨_,_,Sum.inl (.bas nrep bas)⟩ (by simp_all)
+        (fun newPos mov => buildTree s (stillWin newPos mov))
+  | Sum.inl (.nbas nrep nbas) => -- prover chooses a local tableau
+      have stillWin : ∀ newP, ∀ _ : Move ⟨_,_,Sum.inl (.nbas nrep nbas)⟩ newP, winning s newP :=
+        fun newPos mov =>
+          @winning_of_whatever_other_move _ _ s _ (by simp) h ⟨newPos, mem_theMoves_of_move ⟨mov⟩⟩
+      @BuildTree.PrStep ⟨_,_,Sum.inl (.nbas nrep nbas)⟩ (by simp_all)
+        (fun newPos mov => buildTree s (stillWin newPos mov))
+  -- Builder positions:
+  | Sum.inr (.lpr _) => by exfalso; simp [winning] at h -- prover wins, cannot happen
+  | Sum.inr (.ltab nrep nbas ltX) =>
+      if ne : (tableauGame.moves ⟨H, ⟨X, Sum.inr (BuilderPos.ltab nrep nbas ltX)⟩⟩).Nonempty
+      then
+        -- Builder can use `s` to choose some `Y ∈ endNodeOf ltX`.
+        let sY := (s ⟨H, X, Sum.inr (.ltab nrep nbas ltX)⟩ (by simp) ne)
+        have Mov : Move ⟨H, X, Sum.inr (.ltab nrep nbas ltX)⟩ sY.1 := by
+          have := sY.2
+          simp only [Game.Pos.moves, tableauGame, theMoves, List.mem_toFinset] at this
+          simp [List.mem_map] at this
+          let oY := List.find? -- No more choice thanks to this!
+            (fun Y => @decide (⟨X :: H, ⟨Y, posOf (X :: H) Y⟩⟩ = sY.val) (instDecidableEqPos _ _))
+            (endNodesOf ltX)
+          cases oY_def : oY
+          · exfalso
+            have := List.find?_eq_none.mp oY_def
+            grind
+          case some Y =>
+            unfold oY at oY_def
+            have def_sY := List.find?_some oY_def
+            simp only [decide_eq_true_eq] at def_sY
+            have Y_in := List.mem_of_find?_eq_some oY_def
+            have := @Move.buEnd X ltX Y H nrep nbas Y_in
+            rw [← def_sY]
+            exact this
+        have stillWin : winning s sY.1 := winning_of_winning_move _ h
+        have forTermination : move ⟨H, X, Sum.inr (.ltab nrep nbas ltX)⟩ sY.1 := ⟨Mov⟩ -- needed?
+        BuildTree.BuStep (by simp) Mov (buildTree s stillWin)
+      else by
+        exfalso
+        simp_all [winning, winner]
+termination_by
+  tableauGame.wf.2.wrap (⟨H, X, p⟩ : GamePos)
+decreasing_by -- show that it's a move
+  · simp_wf
+    simp only [tableauGame, Game.wf, WellFoundedRelation.rel]
+    exact ⟨mov⟩
+  · simp_wf
+    simp only [tableauGame, Game.wf, WellFoundedRelation.rel]
+    exact ⟨mov⟩
+  · simp_wf
+    simp only [tableauGame, Game.wf, WellFoundedRelation.rel]
+    exact forTermination
+
+/-! ## Matches -/
+
+/-- A match is a path inside a `BuildTree`. Analogous to `PathIn` for `Tableau`. In Game Theory
+this could be called a "rollout", but note that it stays within the given Builder strategy tree. -/
+inductive Match : ∀ {pos : GamePos}, BuildTree pos → Type
+  | nil {bt} : Match bt
+  | bu : Match next → Match (BuildTree.BuStep hturn m next)
+  | pr newPos :
+      (mov : Move pos newPos)
+      → Match (next newPos mov) → Match (@BuildTree.PrStep pos hturn next)
+
+/-
+-- TODO, use `LocalAll` and `AllPdlRule`
+-- Wait, where are these actually used at the moment or will they be needed later?
+
+def BuildTree.all_Match (bt : BuildTree pos) : List (Match bt) := sorry
+
+theorem BuildTree.all_Match_spec (bt : BuildTree pos) :
+    ∀ m, m ∈ bt.all_Match := by
+  sorry
+-/
+
+/-- Inspired by `PathIn.length`.
+Note that this counts all steps, even the `prLocTab` ones where `pos.1` does not get longer. -/
+@[simp]
+def Match.length {pos : GamePos} {bt : BuildTree pos} : Match bt → Nat
+  | .nil => 0
+  | .bu tail => tail.length + 1
+  | .pr _ _ tail => tail.length + 1
+
+def Match.btAt {pos} {bt : BuildTree pos} : Match bt → Σ newPos, BuildTree newPos
+| .nil => ⟨_, bt⟩
+| .bu tail => btAt tail
+| .pr _ _ tail => btAt tail
+
+-- TODO lemmas like those about `tabAt` and `nodeAt`?
+
+def Match.append : (m1 : Match bt) → (m2 : Match (btAt m1).2) → Match bt
+| .nil, m2 => m2
+| .bu tail, m2 => .bu (append tail m2)
+| .pr _ _ tail, m2 => .pr _ _ (append tail m2)
+
+-- TODO lemmas like those about `PathIn.append`?
+
+structure Match.BuEdge (m n : Match bt) where
+  mPos : GamePos
+  hturn : tableauGame.turn mPos = Builder
+  mov : Move mPos n.btAt.1
+  h : btAt m = ⟨mPos, @BuildTree.BuStep _ _ hturn mov (btAt n).2⟩
+
+structure Match.PrEdge (m n : Match bt) where
+  mPos : GamePos
+  hturn : tableauGame.turn mPos = Prover
+  mov : Move mPos n.btAt.1
+  next : _
+  btAt_m_def : btAt m = ⟨mPos, @BuildTree.PrStep _ hturn next⟩
+  next_n_def : next (btAt n).1 n_in = (btAt n).2
+
+/-- The parent-child relation ⋖_𝕋 in a Builder strategy tree. -/
+def Match.Edge (m n : Match bt) : Type := Match.BuEdge m n ⊕ Match.PrEdge m n
+
+/-- This edge between matches is a modal step.
+To even say this `BuildTree` must contain `Move` and thus rule data. -/
+def Match.Edge.isModal {pos} {bt : BuildTree pos} {m n : Match bt} : Match.Edge m n → Prop :=
+  match btAt_m_def : btAt m with
+  | ⟨⟨Hist, X, p⟩, m_bt⟩ =>
+    fun m_n =>
+      match m_bt with
+      | @BuildTree.BuStep _ p YS next YS_moves => False -- Builder moves are never modal steps.
+      | .PrStep hturn next =>
+        match m_n with
+        | .inl m_bu_n => by exfalso; grind [BuEdge]
+        | .inr m_pr_n => m_pr_n.mov.isModal
+
+def Match.isLeaf {pos} {bt : BuildTree pos} {m : Match bt} : Prop := (btAt m).2.isLeaf
+
+/-- If `m` ends at a leaf, then it cannot have an edge to any `n`. -/
+lemma Match.isLeaf_no_edge {bt : BuildTree pos} (m : Match bt) (h : m.isLeaf) :
+    ∀ n, ¬ Nonempty (Match.Edge m n) := by
+  intro n
+  unfold Match.isLeaf at h
+  by_contra hyp
+  rcases hyp with ⟨m_bu_n|m_pr_n⟩
+  · grind [BuildTree.isLeaf, Match.BuEdge]
+  · simp only [BuildTree.isLeaf] at h
+    rcases m_pr_n with ⟨mPos, hturn, mov, next, btAt_m_def, next_n_def⟩
+    have := @mem_theMoves_of_move mPos n.btAt.1 ⟨mov⟩
+    grind
+
+/-- Convert a `Match` to a `History`. Inspired by `PathIn.toHistory`.
+Does not include the last node.
+The history of `.nil` is `[]` because this will not go into `pos.1`.
+IDEA: only record the .pr steps here, but skip .bu steps?!
+-/
+def Match.toHistory {pos : GamePos} {bt : BuildTree pos} : (m : Match bt) → History
+| .nil => []
+| .bu tail => tail.toHistory ++ [pos.2.1]
+| .pr _ _ tail => tail.toHistory ++ [pos.2.1]
+
+/-- Rewind a `Match`, i.e. go back up inside `bt` by `k` steps.
+This used to use `Nat` but now we take a `Fin` like in `PathIn.rewind`, and
+for that we needed to define `Match.length` first.
+IDEA: also use `Match.toHistory` here? -/
+def Match.rewind {pos} {bt : BuildTree pos} : (m : Match bt) → (k : Fin (m.length + 1)) → Match bt
+| .nil, _ => .nil
+| .bu tail, k => Fin.lastCases (.nil) (Match.bu ∘ tail.rewind) k
+| .pr _ _ tail, k => Fin.lastCases (.nil) (Match.pr _ _ ∘ tail.rewind) k
+
+-- ... lots of stuff needed here?
+
+/-- The extra condition that it is the turn of Builder is needed because otherwise
+the `prLocTab` case would falsify. -/
+theorem Move.fst_length_succ {H X p} (mov : Move ⟨H, ⟨X, p⟩⟩ newPos) :
+    tableauGame.turn ⟨H, ⟨X, p⟩⟩ = Builder →
+    newPos.1.length = H.length + 1 := by
+  cases mov <;> simp
+
+/-- This is NOT TRUE, because history only records different steps and will
+*not* count `Move.prLocTab` steps, though these are steps in the `Match`.
+
+WAIT, but `Match.toHistory` DOES count all steps, so the length statement here should be true. ??
+
+?? are we sure about this one ??
+Note that the history from `pos` needs to be added on the right side.
+
+?? Or better restrict `pos` to be a *starting* position of the game!?!?
+(Analogous to how many things in TableauPath are only the `Hist = []` case.) -/
+theorem Match.btAt_fst_fst_length_eq_length {bt : BuildTree pos} {m : Match bt} :
+    m.btAt.1.1.length = m.length + pos.1.length := by
+  induction bt
+  case BuStep pos newPos hturn mov next IH =>
+    cases m
+    case nil =>
+      rcases pos with ⟨H, X, p⟩
+      simp [Match.btAt]
+    case bu hturn tail =>
+      -- FIXME: change defs above to avoid duplicate `hturn` here?!
+      rcases pos with ⟨H, X, p⟩
+      simp [Match.btAt]
+      specialize @IH tail
+      rw [add_assoc]
+      convert IH using 2
+      grind [Move.fst_length_succ mov]
+  case PrStep pos hturn next IH =>
+    cases m
+    case nil =>
+      rcases pos with ⟨H, X, p⟩
+      simp [Match.btAt]
+    case pr newPos hturn mov tail =>
+      rcases pos with ⟨H, X, p⟩
+      simp [Match.btAt]
+      specialize @IH _ mov tail
+      rw [add_assoc]
+      convert IH using 2
+      -- NOT provable here because `newPos.1` is a history not counting `prLocTab` steps,
+      -- whereas the H list coming from `Match.toHistory` does count them.
+      sorry
+
+def Match.companionOf {bt : BuildTree pos} (m : Match bt)
+  (h : (btAt m).2.isFreeRepLeaf) : Match bt :=
+    -- WAS: m.rewind (theRep ((btAt m).2.rep_of_isFreeRepLeaf h))
+    -- WANT: m.rewind (rep.toFin ((btAt m).2.rep_of_isFreeRepLeaf h))
+    sorry
+
+/-- The repeat ♥ companion relation on `Match`. -/
+def Match.companion (m n : Match bt) : Prop :=
+  ∃ (h : (btAt m).2.isFreeRepLeaf), n = Match.companionOf m h
+
+local notation ma:arg " ♥ " mb:arg => Match.companion ma mb
+
+/-! ## Pre-states (Def 6.13)
+
+As possible worlds for the model graph we want to define *maximal* paths inside the build tree
+that do not contain `(M)` steps.
+
+In the paper pre-states are allowed to be of the form π;π' when π ends at a repeat and π' is a
+maximal prefix of the path from the companion to that repeat. Here in `PreState` and `PreStateP`
+we only store the π part of such pre-states, because the π' is then uniquely determined by π.
+-/
+
+/-- A pre-state-part starting at `m` is any path in `bt : BuildTree` consisting of non-(M) `edge`s
+and stopping at a leaf or at an (M) application. (No `Match.companion` steps here, see note above.)
+
+PROBLEM / QUESTION: do we also need leafs given by empty `prMoves`??? -/
+inductive PreStateP {pos} (bt : BuildTree pos) : (m : Match bt) → Type
+| edge {m n} : (e : Match.Edge m n) → ¬ e.isModal → PreStateP bt n → PreStateP bt m
+| stopLeaf {m} : m.isLeaf → PreStateP bt m
+| stopAtM {m n} : (e : Match.Edge m n) → e.isModal → PreStateP bt m
+
+/-- Collect all `PreStateP`s from a given `m` onwards. -/
+def BuildTree.allPreStatePs {pos} : (bt : BuildTree pos) → (m : Match bt) → List (PreStateP bt m)
+  -- Maybe define `Match.all` first and then filter it here?
+  -- Or better do it inductively?
+| .PrStep hturn next, m => sorry
+    -- [ .stopLeaf (by unfold Match.isLeaf; cases m; simp_all [Match.btAt]) ]
+| .BuStep hturn mov next, _ => sorry
+
+lemma BuildTree.allPreStatePs_spec {pos} {bt : BuildTree pos} {m : Match bt} :
+    ∀ π : PreStateP bt m, π ∈ bt.allPreStatePs m := by
+  sorry
+
+/-- A pre-state is a maximal pre-state-part, i.e. starting at the root or just after (M).
+
+WORRY: should `fromRoot` also have a condition about `pos` being the start of the game?
+-/
+inductive PreState {pos} (bt : BuildTree pos) : Type
+| fromRoot : PreStateP bt .nil → PreState bt
+| fromMod {o m} : (e : Match.Edge o m) → e.isModal → PreStateP bt m → PreState bt
+
+/-- Collect all `PreState`s for a given `BuildTree`. -/
+def BuildTree.allPreStates {pos} (bt : BuildTree pos) : List (PreState bt) :=
+  (bt.allPreStatePs .nil).map .fromRoot
+
+lemma BuildTree.allPreStates_spec {pos} {bt : BuildTree pos} :
+    ∀ π : PreState bt, π ∈ bt.allPreStates := by
+  -- should be easy, use BuildTree.allPreStatePs_spec
+  sorry
+
+/-- Collect formulas in a pre-state. The non-loaded part of Λ(π) in paper.
+
+TODO: If the pre-state ends in a repeat, also include formulas in the path from companion to (M).
+
+QUESTION: Can we collect loaded formulas here by unloading them?
+Or would that make the loaded case of `PreState.pdlFormCase` unsayable?
+-/
+def PreState.forms : PreState bt → List Formula := sorry
+
+/-- Collect formulas in a pre-state. The loaded part of Λ(π) in paper. -/
+def PreState.lforms : PreState bt → List NegLoadFormula := sorry
+
+def PreState.last : PreState bt → Sequent := sorry
+
+/-- TODO Lemma 6.14 -/
+lemma PreState.formsCases {π : PreState bt} : φ ∈ π.forms →
+      (φ.basic ∧ φ ∈ π.last) -- NOTE: the `∈` is not dealing with loaded formulas here!
+    ∨ (sorry) := by -- TODO how to say `φ is principal later?`
+    -- Or can we say something else / phrase it as closure condition about π.forms directly?
+  sorry
+
+/-- WIP Lemma 6.15 (unloaded case only) -/
+lemma PreState.pdlFormCase {π : PreState bt} : ¬ α.isAtomic → (~⌈α⌉φ) ∈ π.forms →
+    ∃ Xδ ∈ H α, Xδ.1 ∪ [~ Formula.boxes δ φ] ⊆ π.forms := by
+  sorry
+
+/-- WIP Lemma 6.16: pre-states are saturated and locally consistent, their last node is basic. -/
+lemma PreState.locConsSatBas (π : PreState bt) :
+    saturated (π.forms).toFinset
+    ∧ locallyConsistent (π.forms).toFinset
+    ∧ π.last.basic := by
+  -- define `PreState.forms` first.
+  sorry
+
+/-- Definition 6.17 to get model graph from strategy tree. -/
+@[simp]
+def BuildTree.toModel (bt : BuildTree Pos) : (Σ W : Finset (Finset Formula), KripkeModel W) :=
+  ⟨ ((bt.allPreStates).map (List.toFinset ∘ PreState.forms)).toFinset -- W
+  , { val := fun X p => Formula.atom_prop p ∈ X.1 -- valuation V(p)
+    , Rel := fun a X Y => -- relation Rₐ
+        ∃ φ, (~⌈·a⌉φ) ∈ X.1 ∧ (projection a X.1.toList).toFinset ∪ {~φ} ⊆ Y.1 }⟩
+
+/-- WIP Lemma 6.18
+
+QUESTION: which `R` can we use here in order to use `Modelgraphs.Q`?
+-/
+lemma PreState.diamondExistence {φ : AnyFormula} {π : PreState bt} : (~'⌊α⌋φ) ∈ π.lforms →
+    -- QUESTION: what to say about `π` here and what to say about node `t` lying on `π`?
+    ∃ t : Match bt,
+        AnyNegFormula.mem_Sequent (t.btAt).1.2.1 (~''φ)
+      ∧ ∃ ρ : PreState bt, ∃ u : Match bt,
+        -- TODO: t < u
+        -- TODO: missing loaded formulas below
+        @Modelgraphs.Q sorry sorry α ⟨π.forms.toFinset, sorry⟩ ⟨ρ.forms.toFinset, sorry⟩ := by
+  sorry
+
+-- TODO Lemma 6.19: for any diamond we can go to a pre-state where that diamond is loaded
+
+-- TODO Lemma 6.20: diamond existence lemma for pre-states
+
+/-! ## Model graph of pre-states -/
+
+/-- Theorem 6.21: If Builder has a winning strategy then there is a model graph. -/
+theorem strmg (X : Sequent) (s : Strategy tableauGame Builder) (h : winning s (startPos X)) :
+    ∃ (WS : Finset (Finset Formula)) (mg : ModelGraph WS), ∃ Z ∈ WS, X.toFinset ⊆ Z := by
+  let bt := buildTree s h
+  let WS := bt.toModel.1
+  let M := bt.toModel.2
+  refine ⟨WS, ⟨M, ⟨?a, ?b, ?c, ?d⟩⟩, ?X_in⟩
+  -- show the model graph properties
+  case a =>
+    rintro ⟨X, X_in⟩
+    unfold WS at X_in
+    simp at X_in
+    rcases X_in with ⟨π, in_all, def_X⟩
+    have := PreState.locConsSatBas π-- using Lemma 6.16 for (i)
+    simp_all
+  -- "(b, c) will follow immediately from the definition"
+  case b =>
+    simp_all [M]
+  case c =>
+    intro X Y a φ X_a_Y aφ_in_X -- pick any ⌈a⌉φ
+    simp only [M] at X_a_Y
+    rcases X_a_Y with ⟨ψ, in_X, sub_Y⟩ -- relation was witnessed by ⌈a⌉ψ
+    apply sub_Y -- show that φ is in projection
+    simp_all
+  case d =>
+    simp
+    intro w w_in α φ in_w
+    -- "The main challenge" :-)
+    -- Need Lemmas 6.18 to 6.19 about pre-states here.
+    sorry
+  case X_in =>
+    unfold WS
+    simp
+    -- need actual def for `BuildTree.allPreStates` first
+    -- use the .fromRoot pre-state
+    sorry
